updates for new Cenv_bs, rethinking its definition
need to include the module environment in the invariant saying the
semantic environment matches the machine environment.
however, closure bodies are compiled with respect to a "zero" sized
stack, since before they didn't ever look below the environment and
arguments... now might need another parameter indicating the size of the
real stack below, against which module variables should be looked up...

the implementation may need to change for this too...

compiler/proofs/toBytecodeProofsScript.sml
@@ -206,9 +206,9 @@ val env_renv_def = Define`
      Cenv renv)`
 
 val Cenv_bs_def = Define`
-  Cenv_bs rd Cmenv s Cenv (menv:string|->ctenv) (renv:ctenv) sz bs ⇔
+  Cenv_bs rd Cmenv s Cenv (menv:string|->ctenv) (renv:ctenv) sz mz bs ⇔
     env_renv rd sz bs Cenv renv ∧
-    fmap_rel (env_renv rd sz bs) Cmenv menv ∧
+    fmap_rel (env_renv rd (sz+mz) bs) Cmenv menv ∧
     s_refs rd s bs`
 
 val Cenv_bs_syneq_store = store_thm("Cenv_bs_syneq_store",
@@ -1450,12 +1450,13 @@ val compile_append_out = store_thm("compile_append_out",
   rw[] >> spose_not_then strip_assume_tac >> res_tac >> DECIDE_TAC)
 
 val Cenv_bs_imp_incsz = store_thm("Cenv_bs_imp_incsz",
-  ``∀rd s env renv rsz bs bs'.
-    Cenv_bs rd s env renv rsz bs ∧
+  ``∀rd menv s env rmenv renv rsz bs bs'.
+    Cenv_bs rd menv s env rmenv renv rsz bs ∧
     (∃v p e. (bs' = bs with <| stack := v::bs.stack; pc := p; handler := e |>))
     ⇒
-    Cenv_bs rd s env renv (rsz+1) bs'``,
-  rw[Cenv_bs_def,s_refs_def,good_rd_def] >> rw[] >> fs[] >>
+    Cenv_bs rd menv s env rmenv renv (rsz+1) bs'``,
+  rw[Cenv_bs_def,s_refs_def,good_rd_def,env_renv_def,fmap_rel_def] >> rw[] >> fs[] >>
+  res_tac >>
   match_mp_tac(GEN_ALL(MP_CANON EVERY2_mono)) >>
   HINT_EXISTS_TAC >> simp[] >>
   rpt gen_tac >>
@@ -1463,13 +1464,14 @@ val Cenv_bs_imp_incsz = store_thm("Cenv_bs_imp_incsz",
   imp_res_tac lookup_ct_imp_incsz >>
   simp[])
 
-val Cenv_bs_imp_decsz = store_thm("Cenv_bs_imp_decsz",
-  ``∀rd s env renv rsz bs bs'.
-    Cenv_bs rd s env renv (rsz+1) bs ∧
-      (CTLet (rsz+1) ∉ set renv) ∧
-      (∃v p e. bs = bs' with <| stack := v::bs'.stack; pc := p; handler := e |>) ⇒
-    Cenv_bs rd s env renv rsz bs'``,
-  rw[Cenv_bs_def,fmap_rel_def,s_refs_def,FDOM_DRESTRICT,good_rd_def] >> fs[] >>
+val env_renv_imp_decsz = store_thm("env_renv_imp_decsz",
+  ``∀rd rsz bs env renv bs'.
+    env_renv rd (rsz+1) bs env renv ∧
+    (∃v p e. bs = bs' with <| stack := v::bs'.stack; pc := p; handler := e |>) ∧
+    (CTLet (rsz+1) ∉ set renv)
+    ⇒
+    env_renv rd rsz bs' env renv``,
+  rw[env_renv_def] >> fs[] >>
   fs[EVERY2_EVERY,EVERY_MEM,FORALL_PROD] >>
   rpt strip_tac >> res_tac >> pop_assum mp_tac >>
   BasicProvers.CASE_TAC >>
@@ -1478,36 +1480,60 @@ val Cenv_bs_imp_decsz = store_thm("Cenv_bs_imp_decsz",
   rfs[MEM_ZIP,MEM_EL] >>
   metis_tac[])
 
-val Cenv_bs_CTLet_bound = store_thm("Cenv_bs_CTLet_bound",
-  ``Cenv_bs rd s env renv rsz bs ∧ MEM (CTLet n) renv ⇒ n ≤ rsz``,
-  rw[Cenv_bs_def,EVERY2_EVERY,EVERY_MEM,FORALL_PROD] >>
+val Cenv_bs_imp_decsz = store_thm("Cenv_bs_imp_decsz",
+  ``∀rd menv s env rmenv renv rsz bs bs'.
+    Cenv_bs rd menv s env rmenv renv (rsz+1) bs ∧
+      (CTLet (rsz+1) ∉ set renv) ∧
+      (CTLet (rsz+1) ∉ BIGUNION (IMAGE set (FRANGE rmenv))) ∧
+      (∃v p e. bs = bs' with <| stack := v::bs'.stack; pc := p; handler := e |>) ⇒
+    Cenv_bs rd menv s env rmenv renv rsz bs'``,
+  rw[Cenv_bs_def,fmap_rel_def,s_refs_def,FDOM_DRESTRICT,good_rd_def] >> fs[] >>
+  match_mp_tac env_renv_imp_decsz >>
+  res_tac >> HINT_EXISTS_TAC >>
+  simp[bc_state_component_equality] >>
+  fs[IN_FRANGE] >> metis_tac[])
+
+val env_renv_CTLet_bound = store_thm("env_renv_CTLet_bound",
+  ``env_renv rd rsz bs env renv ∧ CTLet n ∈ set renv ⇒ n ≤ rsz``,
+  rw[EVERY2_EVERY,EVERY_MEM,FORALL_PROD,env_renv_def] >>
   rfs[MEM_ZIP,MEM_EL] >> fsrw_tac[DNF_ss][] >>
-  qmatch_assum_rename_tac `z < LENGTH renv`[]>>
+  qmatch_assum_abbrev_tac `z < LENGTH E`>>
   first_x_assum (qspec_then `z` mp_tac) >>
   qpat_assum`CTLet n = X`(assume_tac o SYM) >>
   simp[el_check_def] >>
   srw_tac[ARITH_ss][])
 
+val Cenv_bs_CTLet_bound = store_thm("Cenv_bs_CTLet_bound",
+  ``Cenv_bs rd menv s env rmenv renv rsz bs ∧ (CTLet n) ∈ set renv ∪ BIGUNION (IMAGE set (FRANGE rmenv)) ⇒ n ≤ rsz``,
+  rw[Cenv_bs_def,fmap_rel_def,IN_FRANGE] >>
+  match_mp_tac (GEN_ALL env_renv_CTLet_bound) >>
+  metis_tac[])
+
 val Cenv_bs_pops = store_thm("Cenv_bs_pops",
-  ``∀vs rd s env renv rsz bs bs'. Cenv_bs rd s env renv (rsz + LENGTH vs) bs ∧
+  ``∀vs rd menv s env rmenv renv rsz bs bs'.
+    Cenv_bs rd menv s env rmenv renv (rsz + LENGTH vs) bs ∧
     (∀n. MEM (CTLet n) renv ⇒ n ≤ rsz) ∧
+    (∀n. (CTLet n) ∈ BIGUNION (IMAGE set (FRANGE rmenv)) ⇒ n ≤ rsz) ∧
     (∃p e. bs = bs' with <| stack := vs ++ bs'.stack; pc := p; handler := e|>)
-    ⇒ Cenv_bs rd s env renv rsz bs'``,
-  Induct >> rw[] >- ( fs[Cenv_bs_def,s_refs_def,good_rd_def] >> fs[]) >>
+    ⇒ Cenv_bs rd menv s env rmenv renv rsz bs'``,
+  Induct >> rw[] >- ( fs[Cenv_bs_def,s_refs_def,good_rd_def,fmap_rel_def,env_renv_def] >> fs[]) >>
   first_x_assum match_mp_tac >>
   simp[bc_state_component_equality] >>
   qexists_tac`bs' with stack := vs ++ bs'.stack` >> rw[] >>
+  fsrw_tac[DNF_ss][] >> TRY(PROVE_TAC[])>>
   match_mp_tac Cenv_bs_imp_decsz >>
-  qmatch_assum_abbrev_tac`Cenv_bs rd s env renv x y` >>
+  qmatch_assum_abbrev_tac`Cenv_bs rd menv s env rmenv renv x y` >>
   qexists_tac`y` >>
   unabbrev_all_tac >>
   fsrw_tac[ARITH_ss][ADD1,bc_state_component_equality] >>
+  conj_tac >>
   spose_not_then strip_assume_tac >>
+  TRY(BasicProvers.VAR_EQ_TAC) >>
   res_tac >> fsrw_tac[ARITH_ss][] )
 
 val Cenv_bs_with_pc = store_thm("Cenv_bs_with_pc",
-  ``Cenv_bs rd s env env0 sz0 (bs with pc := p) = Cenv_bs rd s env env0 sz0 bs``,
-  rw[Cenv_bs_def,s_refs_with_pc])
+  ``Cenv_bs rd menv s rmenv env env0 sz0 (bs with pc := p) = Cenv_bs rd menv s rmenv env env0 sz0 bs``,
+  rw[Cenv_bs_def,env_renv_def,fmap_rel_def,s_refs_with_pc])
 
 val Cv_bv_l2a_mono = store_thm("Cv_bv_l2a_mono",
   ``∀pp.
@@ -1555,11 +1581,11 @@ val s_refs_append_code = store_thm("s_refs_append_code",
   rw[] >> metis_tac[bc_find_loc_aux_append_code])
 
 val Cenv_bs_append_code = store_thm("Cenv_bs_append_code",
-  ``∀rd s env env0 sz0 bs bs' ls.
-    Cenv_bs rd s env env0 sz0 bs ∧ (bs' = (bs with code := bs.code ++ ls)) ⇒
-    Cenv_bs rd s env env0 sz0 bs'``,
+  ``∀rd menv s rmenv env env0 sz0 bs bs' ls.
+    Cenv_bs rd menv s rmenv env env0 sz0 bs ∧ (bs' = (bs with code := bs.code ++ ls)) ⇒
+    Cenv_bs rd menv s rmenv env env0 sz0 bs'``,
   reverse(rw[Cenv_bs_def]) >- PROVE_TAC[s_refs_append_code] >>
-  fs[Cenv_bs_def,EVERY2_EVERY,EVERY_MEM,FORALL_PROD,s_refs_def] >> rw[] >>
+  fs[Cenv_bs_def,EVERY2_EVERY,EVERY_MEM,FORALL_PROD,s_refs_def,env_renv_def,fmap_rel_def] >> rw[] >>
   res_tac >>
   BasicProvers.CASE_TAC >> fs[] >>
   match_mp_tac Cv_bv_l2a_mono_mp >>
@@ -1567,30 +1593,29 @@ val Cenv_bs_append_code = store_thm("Cenv_bs_append_code",
   rw[] >> metis_tac[bc_find_loc_aux_append_code])
 
 val Cenv_bs_FUPDATE = store_thm("Cenv_bs_FUPDATE",
-  ``∀rd s env env0 sz0 bs v bv bs'.
-    Cenv_bs rd s env env0 sz0 bs ∧
+  ``∀rd menv s env env0 rmenv sz0 bs v bv bs'.
+    Cenv_bs rd menv s env rmenv env0 sz0 bs ∧
     Cv_bv (mk_pp rd bs') v bv ∧
     (bs' = bs with stack := bv::bs.stack)
     ⇒
-    Cenv_bs rd s (v::env) ((CTLet (sz0 + 1))::env0) (sz0 + 1) bs'``,
-  rw[Cenv_bs_def,s_refs_def] >> fs[el_check_def] >- (
-    fs[EVERY2_EVERY,EVERY_MEM,FORALL_PROD] >>
-    rpt strip_tac >> res_tac >>
-    pop_assum mp_tac >> BasicProvers.CASE_TAC >>
-    imp_res_tac lookup_ct_imp_incsz >>
-    simp[] ) >>
-  fs[good_rd_def])
+    Cenv_bs rd menv s (v::env) rmenv ((CTLet (sz0 + 1))::env0) (sz0 + 1) bs'``,
+  reverse(rw[Cenv_bs_def,s_refs_def]) >> fs[el_check_def] >- fs[good_rd_def] >> (
+  fs[EVERY2_EVERY,EVERY_MEM,FORALL_PROD,env_renv_def,fmap_rel_def,el_check_def] >>
+  rpt strip_tac >> res_tac >>
+  pop_assum mp_tac >> BasicProvers.CASE_TAC >>
+  imp_res_tac lookup_ct_imp_incsz >>
+  simp[] ))
 
 val Cenv_bs_FUPDATE_LIST = store_thm("Cenv_bs_FUPDATE_LIST",
-  ``∀vs rd s env cenv sz bs bs bvs bs' env' cenv' sz'.
-  Cenv_bs rd s env cenv sz bs ∧
+  ``∀vs rd menv s env rmenv cenv sz bs bs bvs bs' env' cenv' sz'.
+  Cenv_bs rd menv s env rmenv cenv sz bs ∧
   (bs' = bs with stack := bvs ++ bs.stack) ∧
   EVERY2 (Cv_bv (mk_pp rd bs')) vs bvs ∧
   (env' = vs++env) ∧
   (cenv' = (REVERSE(GENLIST(λm. CTLet(sz+m+1))(LENGTH vs)))++cenv) ∧
   (sz' = sz + LENGTH vs)
   ⇒
-  Cenv_bs rd s env' cenv' sz' bs'``,
+  Cenv_bs rd menv s env' rmenv cenv' sz' bs'``,
   Induct >- (
     simp[LENGTH_NIL,FUPDATE_LIST_THM] ) >>
   rw[] >>
@@ -1612,22 +1637,21 @@ val Cenv_bs_FUPDATE_LIST = store_thm("Cenv_bs_FUPDATE_LIST",
   simp[])
 
 val Cenv_bs_DOMSUB = store_thm("Cenv_bs_DOMSUB",
-  ``∀rd s env renv rsz bs.
-    Cenv_bs rd s env renv rsz bs ∧ (env ≠ []) ∧ (renv ≠ []) ⇒
-    Cenv_bs rd s (TL env) (TL renv) rsz bs``,
-  ntac 2 gen_tac >> Cases >> simp[] >> Cases >> simp[] >>
-  rw[Cenv_bs_def,EVERY2_EVERY])
+  ``∀rd menv s env rmenv renv rsz bs.
+    Cenv_bs rd menv s env rmenv renv rsz bs ∧ (env ≠ []) ∧ (renv ≠ []) ⇒
+    Cenv_bs rd menv s (TL env) rmenv (TL renv) rsz bs``,
+  ntac 3 gen_tac >> Cases >> simp[] >> gen_tac >> Cases >> simp[] >>
+  rw[Cenv_bs_def,EVERY2_EVERY,env_renv_def,fmap_rel_def])
 
-val Cenv_bs_change_store = store_thm("Cenv_bs_change_store",
-  ``∀rd s env renv rsz bs rd' s' bs' rfs'.
-    Cenv_bs rd s env renv rsz bs ∧
-    s_refs rd' s' bs' ∧
-    (bs' = bs with refs := rfs') ∧
-    DRESTRICT bs.refs (COMPL (set rd.sm)) ⊑ DRESTRICT rfs' (COMPL (set rd'.sm)) ∧
-    rd.sm ≼ rd'.sm ∧ rd.cls ⊑ rd'.cls
+val env_renv_change_store = store_thm("env_renv_change_store",
+  ``env_renv rd rsz bs env renv ∧
+    s_refs rd s bs ∧
+    s_refs rd' s' (bs with refs := rfs') ∧
+    rd.sm ≼ rd'.sm ∧ rd.cls ⊑ rd'.cls ∧
+    DRESTRICT bs.refs (COMPL (set rd.sm)) ⊑ DRESTRICT rfs' (COMPL (set rd'.sm))
     ⇒
-    Cenv_bs rd' s' env renv rsz bs'``,
-  rw[Cenv_bs_def,EVERY2_EVERY,EVERY_MEM,FORALL_PROD] >>
+    env_renv rd' rsz (bs with refs := rfs') env renv``,
+  rw[env_renv_def,EVERY2_EVERY,EVERY_MEM,FORALL_PROD] >>
   res_tac >> pop_assum mp_tac >> BasicProvers.CASE_TAC >> strip_tac >>
   qho_match_abbrev_tac`case X of NONE => F | SOME Y => Z Y` >>
   qmatch_assum_abbrev_tac`X' = SOME x` >>
@@ -1644,6 +1668,19 @@ val Cenv_bs_change_store = store_thm("Cenv_bs_change_store",
   simp[] >>
   fs[s_refs_def,good_rd_def,FEVERY_DEF,UNCURRY] >>
   fs[SUBMAP_DEF,SUBSET_DEF,DRESTRICT_DEF,IN_FRANGE] )
+
+val Cenv_bs_change_store = store_thm("Cenv_bs_change_store",
+  ``∀rd menv s env rmenv renv rsz bs rd' s' bs' rfs'.
+    Cenv_bs rd menv s env rmenv renv rsz bs ∧
+    s_refs rd' s' bs' ∧
+    (bs' = bs with refs := rfs') ∧
+    DRESTRICT bs.refs (COMPL (set rd.sm)) ⊑ DRESTRICT rfs' (COMPL (set rd'.sm)) ∧
+    rd.sm ≼ rd'.sm ∧ rd.cls ⊑ rd'.cls
+    ⇒
+    Cenv_bs rd' menv s' env rmenv renv rsz bs'``,
+  rw[Cenv_bs_def,EVERY2_EVERY,EVERY_MEM,FORALL_PROD,fmap_rel_def] >>
+  match_mp_tac (GEN_ALL env_renv_change_store) >>
+  metis_tac[])
 
 val retbc_thm = store_thm("retbc_thm",
   ``∀bs bc0 bc1 bv vs benv ret args x st bs'.
@@ -1776,12 +1813,12 @@ val jmpbc_thm = store_thm("jmpbc_thm",
   rw[])
 
 val code_for_push_def = Define`
-  code_for_push rd bs bce bc0 code s s' env vs renv rsz =
+  code_for_push rd menv bs bce bc0 code s s' env vs rmenv renv rsz =
     ∃bvs rf rd'.
     let bs' = bs with <| stack := (REVERSE bvs)++bs.stack; pc := next_addr bs.inst_length (bc0 ++ code); refs := rf |> in
     bc_next^* bs bs' ∧
     EVERY2 (Cv_bv (mk_pp rd' (bs' with code := bce))) vs bvs ∧
-    Cenv_bs rd' s' env renv (rsz+(LENGTH vs)) (bs' with code := bce) ∧
+    Cenv_bs rd' menv s' env rmenv renv (rsz+(LENGTH vs)) (bs' with code := bce) ∧
     DRESTRICT bs.refs (COMPL (set rd.sm)) ⊑ DRESTRICT rf (COMPL (set rd'.sm)) ∧
     rd.sm ≼ rd'.sm ∧ rd.cls ⊑ rd'.cls`
 
@@ -1796,8 +1833,8 @@ val code_for_return_def = Define`
     rd.sm ≼ rd'.sm ∧ rd.cls ⊑ rd'.cls`
 
 val code_for_push_return = store_thm("code_for_push_return",
-  ``∀rd bs bce bc0 code s s' env v renv rsz bc1 args args1 bs' blvs benv st cl cl1 ret hdl.
-    code_for_push rd bs bce bc0 code s s' env [v] renv rsz ∧
+  ``∀rd menv bs bce bc0 code s s' env v rmenv renv rsz bc1 args args1 bs' blvs benv st cl cl1 ret hdl.
+    code_for_push rd menv bs bce bc0 code s s' env [v] rmenv renv rsz ∧
     (bs.code = bc0 ++ code ++ retbc (LENGTH args) (LENGTH blvs) ++ bc1) ∧
     (bs.stack = blvs++benv::CodePtr ret::args++cl::st) ∧
     (bs.handler = hdl)
@@ -1883,7 +1920,8 @@ val compile_bindings_thm = store_thm("compile_bindings_thm",
   simp[FUN_EQ_THM])
 
 val Cenv_bs_bind_fv = store_thm("Cenv_bs_bind_fv",
-  ``∀cenv ccenv benv bve ret bvs a st fenv defs ix recs envs env pp rd bs s vs az e l e'.
+  ``∀menv rmenv cenv ccenv benv bve ret bvs a st fenv defs ix recs envs env pp rd rsz bs s vs az e l e'.
+    fmap_rel (env_renv rd rsz bs) menv rmenv ∧ rsz ≤ LENGTH st ∧
     (cenv = MAP CTEnv ccenv) ∧
     (benv = Block 0 bve) ∧
     (bs.stack = benv::CodePtr ret::(REVERSE bvs)++(Block closure_tag [CodePtr a;benv])::st) ∧
@@ -1896,9 +1934,9 @@ val Cenv_bs_bind_fv = store_thm("Cenv_bs_bind_fv",
     (FST(EL ix defs) = SOME (l,ccenv,recs,envs)) ∧
     (bc_find_loc_aux bs.code bs.inst_length l 0 = SOME a) ∧
     EVERY2 (Cv_bv pp) vs bvs ∧ (az = LENGTH vs)
-    ⇒ Cenv_bs rd s env cenv 0 bs``,
+    ⇒ Cenv_bs rd menv s env rmenv cenv 0 bs``,
   rw[Cenv_bs_def] >>
-  simp[EVERY2_EVERY] >>
+  simp[env_renv_def,EVERY2_EVERY] >>
   conj_asm1_tac >- (
     fsrw_tac[ARITH_ss][bind_fv_def,LET_THM] >>
     srw_tac[ARITH_ss][]) >>
